renamed partial_fuel* predicates to be consistent with has_fuel*

fairness/resources.v
@@ -795,8 +795,8 @@ Section PartialOwnership.
   Class PartialModelPredicates := {
       partial_model_is: fmstate iM -> iProp Σ;
       partial_free_roles_are: gset (fmrole iM) → iProp Σ;
-      partial_fuel_is: locale Λ → fmrole iM → nat → iProp Σ;
-      partial_fuels_are: locale Λ → gmap (fmrole iM) nat → iProp Σ;
+      partial_fuel: locale Λ → fmrole iM → nat → iProp Σ;
+      partial_fuels: locale Λ → gmap (fmrole iM) nat → iProp Σ;
       partial_thread_disabled: locale Λ → iProp Σ;
       project_inner: M -> iM;
 
@@ -812,15 +812,15 @@ Section PartialOwnership.
           (* (live_roles _ (trace_last auxtr)) ∩ rem = ∅ → *)
           (* rem ⊆ dom fs → *)
           locale_step (trace_last extr) (Some ζ) c2 ->
-          (* partial_fuels_are_S ζ fs -∗ *)
-          partial_fuels_are ζ (S <$> fs) -∗
+          (* partial_fuels_S ζ fs -∗ *)
+          partial_fuels ζ (S <$> fs) -∗
           model_state_interp (trace_last extr).1 (trace_last auxtr)
           ==∗
           ∃ δ2 (ℓ : mlabel LM),
           ⌜labels_match (LM:=LM) (Some ζ) ℓ ∧
             valid_state_evolution_fairness (extr :tr[Some ζ]: c2) (auxtr :tr[ℓ]: δ2)⌝ ∗
           (* has_fuels ζ (fs ⇂ (dom fs ∖ rem)) ∗ *)
-          partial_fuels_are ζ (fs ⇂ (dom fs ∖ ∅)) ∗
+          partial_fuels ζ (fs ⇂ (dom fs ∖ ∅)) ∗
           model_state_interp c2.1 δ2;
 
       update_fork_split: 
@@ -833,10 +833,10 @@ Section PartialOwnership.
     trace_last extr = (tp1, σ1) ->
     locale_step (tp1, σ1) (Some ζ) (tp2, σ2) ->
     (∃ tp1', tp2 = tp1' ++ [efork] ∧ length tp1' = length tp1) ->
-    (* partial_fuels_are_S ζ fs -∗ *)
-    partial_fuels_are ζ (S <$> fs) -∗
+    (* partial_fuels_S ζ fs -∗ *)
+    partial_fuels ζ (S <$> fs) -∗
       model_state_interp (trace_last extr).1 (trace_last auxtr) ==∗
-      ∃ δ2, partial_fuels_are (locale_of tp1 efork) (fs ⇂ R2) ∗ partial_fuels_are ζ (fs ⇂ R1) ∗ model_state_interp tp2 δ2
+      ∃ δ2, partial_fuels (locale_of tp1 efork) (fs ⇂ R2) ∗ partial_fuels ζ (fs ⇂ R1) ∗ model_state_interp tp2 δ2
         ∧ ⌜valid_state_evolution_fairness (extr :tr[Some ζ]: (tp2, σ2)) (auxtr :tr[Silent_step ζ]: δ2)⌝;
 
      update_step_still_alive: 
@@ -851,24 +851,24 @@ Section PartialOwnership.
     trace_last auxtr = δ1 ->
     locale_step (tp1, σ1) (Some ζ) (tp2, σ2) ->
     fmtrans _ s1 (Some ρ) s2 -> valid_new_fuelmap fs1 fs2 (project_inner δ1) s2 ρ (LM := iLM) ->
-    partial_fuels_are ζ fs1 -∗ partial_model_is s1 -∗ model_state_interp tp1 δ1 -∗
+    partial_fuels ζ fs1 -∗ partial_model_is s1 -∗ model_state_interp tp1 δ1 -∗
     partial_free_roles_are fr1
     ==∗ ∃ (δ2: LM) ℓ,
         ⌜labels_match (Some ζ) ℓ
         ∧ valid_state_evolution_fairness (extr :tr[Some ζ]: (tp2, σ2)) (auxtr :tr[ℓ]: δ2)⌝
-        ∗ partial_fuels_are ζ fs2 ∗ partial_model_is s2 ∗ model_state_interp tp2 δ2 ∗
+        ∗ partial_fuels ζ fs2 ∗ partial_model_is s2 ∗ model_state_interp tp2 δ2 ∗
         partial_free_roles_are (fr1 ∖ (live_roles _ s2 ∖ live_roles _ s1));
 
-    partial_fuels_are_Proper :> Proper (equiv ==> equiv ==> equiv) partial_fuels_are;
-    partial_fuel_fuels: forall ζ ρ f, partial_fuel_is ζ ρ f ⊣⊢ partial_fuels_are ζ {[ρ := f]};
+    partial_fuels_Proper :> Proper (equiv ==> equiv ==> equiv) partial_fuels;
+    partial_fuel_fuels: forall ζ ρ f, partial_fuel ζ ρ f ⊣⊢ partial_fuels ζ {[ρ := f]};
     partial_model_agree': forall n δ1 s2,
         model_state_interp n δ1 -∗ partial_model_is s2 -∗ ⌜project_inner δ1 = s2⌝;
     partial_no_fuels_disabled:
-        forall tid, partial_fuels_are tid ∅ -∗ partial_thread_disabled tid;
+        forall tid, partial_fuels tid ∅ -∗ partial_thread_disabled tid;
 
     partial_model_is_Timeless :> forall s, Timeless (partial_model_is s);
-    partial_fuel_is_Timeless :> forall τ ρ f, Timeless (partial_fuel_is τ ρ f);
-    partial_fuels_are_Timeless :> forall τ fs, Timeless (partial_fuels_are τ fs);
+    partial_fuel_Timeless :> forall τ ρ f, Timeless (partial_fuel τ ρ f);
+    partial_fuels_Timeless :> forall τ fs, Timeless (partial_fuels τ fs);
     partial_free_roles_are_Timeless :> forall s, Timeless (partial_free_roles_are s);
   }.
 
@@ -876,38 +876,38 @@ Section PartialOwnership.
     Context {PMP: PartialModelPredicates}. 
 
     (* TODO: is it possible to use it already in class definition? *)
-    Definition partial_fuels_are_S ζ fs := partial_fuels_are ζ (S <$> fs).
+    Definition partial_fuels_S ζ fs := partial_fuels ζ (S <$> fs).
 
-    Definition partial_fuels_are_plus n ζ (fs: gmap (fmrole iM) nat): iProp Σ :=
-      partial_fuels_are ζ (fmap (fun m => n+m) fs).
+    Definition partial_fuels_plus n ζ (fs: gmap (fmrole iM) nat): iProp Σ :=
+      partial_fuels ζ (fmap (fun m => n+m) fs).
 
     Lemma partial_fuel_fuels_plus_1 (ζ: locale Λ) fs:
-      partial_fuels_are_plus 1 ζ fs ⊣⊢ partial_fuels_are_S ζ fs.
+      partial_fuels_plus 1 ζ fs ⊣⊢ partial_fuels_S ζ fs.
     Proof.
-      rewrite /partial_fuels_are_plus /partial_fuels_are_S. do 2 f_equiv.
+      rewrite /partial_fuels_plus /partial_fuels_S. do 2 f_equiv.
       intros m m' ->. apply leibniz_equiv_iff. lia.
     Qed.
 
     Lemma partial_fuel_fuels_plus_0 (ζ: locale Λ) fs:
-      partial_fuels_are_plus 0 ζ fs ⊣⊢ partial_fuels_are ζ fs.
+      partial_fuels_plus 0 ζ fs ⊣⊢ partial_fuels ζ fs.
     Proof.
-      rewrite /partial_fuels_are_plus /=.  f_equiv. intros ?.
+      rewrite /partial_fuels_plus /=.  f_equiv. intros ?.
       rewrite lookup_fmap. apply leibniz_equiv_iff.
       destruct (fs !! i) eqn:Heq; rewrite Heq //.
     Qed.
 
-    Lemma partial_fuels_are_plus_split_S n (ζ: locale Λ) fs:
-      partial_fuels_are_plus (S n) ζ fs ⊣⊢ partial_fuels_are_S ζ ((λ m, n + m) <$> fs).
+    Lemma partial_fuels_plus_split_S n (ζ: locale Λ) fs:
+      partial_fuels_plus (S n) ζ fs ⊣⊢ partial_fuels_S ζ ((λ m, n + m) <$> fs).
     Proof.
-      rewrite /partial_fuels_are_plus /partial_fuels_are_S. f_equiv.
+      rewrite /partial_fuels_plus /partial_fuels_S. f_equiv.
       rewrite -map_fmap_compose /= => ρ.
       rewrite !lookup_fmap //.
     Qed.
 
     Lemma partial_fuel_fuels_S:
-      forall ζ ρ f, partial_fuel_is ζ ρ (S f) ⊣⊢ partial_fuels_are_S ζ {[ρ := f]}.
+      forall ζ ρ f, partial_fuel ζ ρ (S f) ⊣⊢ partial_fuels_S ζ {[ρ := f]}.
     Proof using. 
-      intros. rewrite /partial_fuels_are_S.
+      intros. rewrite /partial_fuels_S.
       rewrite partial_fuel_fuels.
       rewrite map_fmap_singleton //.
     Qed. 
@@ -1625,8 +1625,8 @@ Qed.
     refine {|
         partial_model_is := frag_model_is;
         partial_free_roles_are := frag_free_roles_are;
-        partial_fuel_is := has_fuel;
-        partial_fuels_are := has_fuels;
+        partial_fuel := has_fuel;
+        partial_fuels := has_fuels;
         project_inner := id;
         partial_thread_disabled := fun τ => τ ↦M ∅;
       |}. 
